Working on EQ proof

ovn/proofs/ssprove/extraction/ovn_eq_proof.v
@@ -1,3 +1,225 @@
+Set Warnings "-notation-overridden,-ambiguous-paths".
+From mathcomp Require Import all_ssreflect.
+
+From JasminSSProve Require Import jasmin_translate.
+From Crypt Require Import Prelude Package pkg_composition.
+From Crypt Require Import Axioms. (* proof_irrelevance *)
+From extructures Require Import ord fset fmap.
+Import PackageNotation.
+
+#[global] Hint Resolve preceq_I preceq_O preceq_refl : preceq.
+
+Definition pdisj (P : precond) (s_id : p_id) (rhs : {fset Location}) :=
+  (forall h1 h2 l a v s_id', l = translate_var s_id' v -> (s_id ⪯ s_id') -> (P (h1, h2) -> P (set_heap h1 l a, h2))) /\
+    (forall h1 h2 l a, l \in rhs -> (P (h1, h2) -> P (h1, set_heap h2 l a))).
+
+(* From Crypt Require Import choice_type Package Prelude. *)
+
+Require Import Hacspec_ovn_Schnorr_Random_oracle.
+
+Require Import SigmaProtocol.
+Require Import DDH.
+
+Require Import Hacspec_ovn_Schnorr.
+
+Require Import Schnorr.
+
 Require Import Hacspec_ovn.
-From Crypt Require Import choice_type Package Prelude.
+
+From Hacspec Require Import ChoiceEquality.
+(* From Hacspec Require Import Hacspec_Lib_Pre. *)
+From Hacspec Require Import Hacspec_Lib.
+
+Module Schnorr_eq (GP : GroupParam).
+  Import GP.
+  Module Sigma1 := Schnorr GP.
+  Module RO1 := Sigma1.Sigma.Oracle.
+
+  Check both_prog.
+
+  (* Check (chProd Sigma1.MyAlg.choiceStatement Sigma1.MyAlg.choiceWitness). *)
+  Locate choiceTranscript.
+
+  Definition Schnorr_translate_type (x : Sigma1.MyAlg.choiceStatement × Sigma1.MyAlg.choiceWitness) : t_Relation :=
+    (Hacspec_Lib_Pre.repr _ (word.modulus (nat_of_ord (fst x))),
+      Hacspec_Lib_Pre.repr _ (word.modulus (nat_of_ord (snd x) ))).
+
+  Ltac destruct_pre :=
+    repeat
+      match goal with
+      | [ H : set_lhs _ _ _ _ |- _ ] =>
+          let sn := fresh in
+          let Hsn := fresh in
+          destruct H as [sn [Hsn]]
+      | [ H : set_rhs _ _ _ _ |- _ ] =>
+          let sn := fresh in
+          let Hsn := fresh in
+          destruct H as [sn [Hsn]]
+      | [ H : _ /\ _ |- _ ] =>
+          let H1 := fresh in
+          let H2 := fresh in
+          destruct H as [H1 H2]
+      | [ H : (_ ⋊ _) _ |- _ ] =>
+          let H1 := fresh in
+          let H2 := fresh in
+          destruct H as [H1 H2]
+      | [ H : exists _, _ |- _ ] =>
+          let o := fresh in
+          destruct H as [o]
+      end; simpl in *; subst.
+
+  Ltac remove_get_in_lhs :=
+    eapply better_r_get_remind_lhs ;
+    unfold Remembers_lhs , rem_lhs ;
+    [ intros ? ? ? ;
+      destruct_pre ;
+      repeat (rewrite get_set_heap_neq ; [ | apply injective_translate_var3 ; reflexivity ]) ;
+      rewrite get_set_heap_eq ;
+      reflexivity | ].
+
+  From Crypt Require Import Axioms.
+
+  Check proof_irrelevance.
+
+  Lemma both_eq : forall {A : choice_type} {L I} (a b : both L I A),
+      both_prog a = both_prog b ->
+      a = b.
+  Proof.
+    intros.
+    destruct a , b.
+    cbn in *. subst.
+    f_equal ; apply proof_irrelevance.
+  Qed.
+
+  Lemma bind_ret_both : forall {A B : choice_type} {L I} `{fsubset_loc : is_true (fsubset (fset [::]) L)} `{fsubset_opsig : is_true (fsubset (fset [::]) I)} (f : A -> both L I B) (x : A),
+      (bind_both (fsubset_loc := fsubset_loc) (fsubset_opsig := fsubset_opsig) (ret_both x) f) = f x.
+  Proof.
+    intros.
+    apply both_eq.
+    simpl.
+    unfold bind_raw_both.
+    simpl.
+    destruct (f x). simpl.
+    destruct both_prog. simpl.
+    reflexivity.
+  Qed.
+  
+  Theorem Schnorr_eq_proof id0 (pre : precond)  :
+    forall (hw : (Sigma1.MyAlg.choiceStatement × Sigma1.MyAlg.choiceWitness)),
+    (pdisj pre id0 (fset0)) ->
+    ⊢ ⦃ pre ⦄
+        is_state (both_prog (fiat_shamir_run (ret_both (Schnorr_translate_type hw))))
+        ≈
+        get_op_default (Sigma1.Sigma.Fiat_Shamir ∘ RO1.RO) (Sigma1.Sigma.RUN, ((chProd Sigma1.MyAlg.choiceStatement Sigma1.MyAlg.choiceWitness), Sigma1.MyAlg.choiceTranscript)) hw
+        ⦃ fun '(v0, h0) '(v1, h1) => pre (h0, h1) ⦄.
+  Proof.
+    intros.
+    
+    (* Unfolding and simplifying to raw code! *)
+    (* TODO: Work on higher level than raw code? *)
+    
+    rewrite get_op_default_link.
+    erewrite get_op_default_spec.
+    2: {
+      cbn.
+      done.
+    }
+    ssprove_code_simpl.
+
+    rewrite fiat_shamir_run_equation_1.
+    destruct hw.
+
+    ssprove_code_simpl.
+    ssprove_code_simpl_more.
+
+    unfold let_both at 1.
+
+    unfold prod_to_prod_n at 1 ; fold @prod_to_prod_n ; rewrite prod_to_prod_equation_1 ; rewrite !bind_ret_both ; simpl.
+    unfold Schnorr_translate_type ; simpl.
+    rewrite v_Commit_equation_1.
+
+    unfold Build_t_G at 1.
+
+    
+    unfold is_state , both_prog.
+    rewrite !let_both_equation_1.
+    unfold both_prog.
+    rewrite !prod_both_equation_1.
+    setoid_rewrite bind_assoc.
+    setoid_rewrite bind_assoc.
+    setoid_rewrite bind_assoc.
+    setoid_rewrite bind_assoc.
+    (* unfold is_state, ret_both, lift_both, both_prog, bind_both, bind_raw_both. *)
+
+    (* Actual proof *)
+
+    match goal with
+    | [ |- context [ ⊢ ⦃ ?P ⦄ ?x ≈ assertD ?b ?f ⦃ ?Q ⦄ ] ] =>
+        change x with (assertD true (fun _ => x)) ;
+        apply (r_assertD true b pre _ (fun _ => x))
+    end.
+    {
+      intros.
+      admit.
+    }
+    intros.
+    
+    match goal with
+    | [ |- context [ ⊢ ⦃ ?P ⦄ bind ?a ?f ≈ pkg_core_definition.sampler ?x ?y ⦃ ?Q ⦄ ] ] =>
+        set (a) ; set (f) ; set (x) ; set (y)
+    end.
+    Check pkg_core_definition.sampler o.
+    pose (Arit o).
+    cbn in t.
+    pose Sigma1.MyAlg.i_witness.
+    cbn in n.
+    
+    assert (s1 : forall (x : Arit o), commit_loc).
+    { clear. intros.
+      apply (Schnorr_translate_type).
+      split.
+      (* apply (Hacspec_Lib_Pre.repr _ (word.modulus 1%nat)). *)
+      2:{
+        apply x.
+      }.
+      admit.
+    }
+    replace (x ← r ;; r0 _) with (x ← sample o ;; r0 (s1 x)) by admit.
+    apply r_uniform_bij with (f := id).
+    {
+      apply injF_bij.
+      apply inj_id.
+    }
+    intros.
+    subst r0 r1.
+    hnf.
+
+    
+    Set Printing Coercions.
+    Unset Printing Notations.
+    
+    pose (r_bind).
+    
+    apply r_bind.
+    
+    bind_jazz_bind.
+    
+    
+    
+    apply r_assertR.
+    r_assertR.
+    
+    rewrite bind_assoc.
+    rewrite bind_assoc.
+
+    r_assertR.
+
+    ssprove_sync_eq.
+
+    
 Require Import OVN.
+
+(* Exec_i_realised *)
+(* {package (Exec_i i j m) ∘ (par ((P_i i b) ∘ (Sigma1.Sigma.Fiat_Shamir ∘ RO1.RO)) *)
+(*                                       (Sigma1.Sigma.Fiat_Shamir ∘ RO1.RO))} *)
+
